updated cyril's files and starting typing

theories/Typing.v
@@ -3,10 +3,13 @@ Require Export Arith.
 Require Export Compare_dec.
 Require Export Relations.
 Require Import ssrnat ssrfun ssrbool eqtype seq choice.
+Require Import ordtype finmap.
 Require Import Utf8.
 Set Implicit Arguments.
 Unset Strict Implicit.
 Unset Printing Implicit Defensive.
+
+Open Scope SEQ.
 
 Require Import TermEvar.
 
@@ -16,16 +19,13 @@ Notation type := term.
 (** Typing local context *) 
 Definition ctx := list type.
 
-Definition evar_context := list (ident * (option term * type)).
+Notation odef := (option term * type)%type.
+Definition evar_context := list (ident * odef).
 
 Inductive evar_decl : Set := 
   { evar_ctx : evar_context;
     evar_body : option term;
     evar_concl : type }.
-
-Definition evar_map : Set :=
-  nat -> option evar_decl.
-
 
 Fixpoint closedn (n : nat) (t : term) : bool := 
   match t with
@@ -67,8 +67,6 @@ Definition evar_decl_fevs evd :=
   fevs evd.(evar_concl) ++
   oapp fevs [::] evd.(evar_body).
 
-Definition evar_map_fevs (e : evar_map) : list nat := [::].
-
 Definition wf_term (t : term) := 
   closed t.
 
@@ -97,10 +95,225 @@ Definition wf_evar_decl evd :=
   owf_open_term ctx evd.(evar_body) &&
   wf_open_term ctx evd.(evar_concl).
 
-Definition wf_evar_map (m : evar_map) :=
-  let mfevs := evar_map_fevs m in
-  forall k, if m k is Some x then 
-              wf_evar_decl x && incl (evar_decl_fevs x) mfevs
-            else false.
+Import Order.Theory.
+Notation evar_map := {fmap nat -> evar_decl}.
 
-                                    
+Notation named_ctx := evar_context.
+Notation local_ctx := (seq odef).
+
+Notation def_elem := (None, Srt prop).
+
+Fixpoint oget_def (N : named_ctx) (i : ident) : option odef :=
+  match N with
+  | [::] => None
+  | ((j, e) :: N') => if i == j then Some e else oget_def N' i
+  end.
+
+Definition get_def (d : odef) (N : named_ctx) (i : ident) : odef :=
+  if oget_def N i is Some def then def else d.
+
+Notation "'[db' s ']' t" := (subst s t) (at level 20).
+
+Reserved Notation "'[n' x ':=' t1 ']' t2" (at level 40).
+
+Fixpoint nsubs x t1 t2 :=
+  match t2 with
+    | Srt _ | Bnd _ => t2
+    | Ref i => if i == x then t1 else t2
+    | Op b t u => 
+      Op b ([n x:=t1]t) ([n x:=t1]u)
+    | Evar n l => Evar n (map (nsubs x t1) l)
+  end
+where "'[n' x ':=' t1 ']' t2" := (nsubs x t1 t2).
+
+Fixpoint nmulti_subs (n : named_ctx) (s : seq term) t :=
+  match n, s with
+    | [::], [::] => Some t
+    | ((x, _) :: n'), (t' :: s') => nmulti_subs n' s' ([n x:=t']t)
+    | _ , _ => None
+  end.
+
+Notation "'[n' l '::=' t1 ']' t2" := (nmulti_subs l t1 t2) (at level 40).
+
+Reserved Notation "E '||-' t '~' T" (at level 40).
+Reserved Notation "E '||-*' s '~' c" (at level 40).
+
+Reserved Notation "E '||-' t1 '-->' t2" (at level 40).
+
+Inductive red1 : (evar_map * named_ctx * local_ctx) -> term -> term -> Prop :=
+  | beta C M N T : C ||- App (Abs T M) N --> subst N M
+  | deltaN E N L i t T :
+      oget_def N i = Some (Some t, T) ->
+      (E, N, L) ||- Ref i --> t
+  | deltaL E N L n t T : 
+      n < size L -> nth def_elem L n = (Some t, T) ->
+      (E, N, L) ||- Bnd n --> t
+  | deltaE E N L e s d b b':
+      E.[e] = Some d -> d.(evar_body) = Some b ->
+      [n d.(evar_ctx) ::= s]b = Some b' ->
+      (E, N, L) ||- Evar e s --> b'
+  | red1l (b : op) C M M' N : 
+      C ||- M --> M' -> 
+      C ||- b M N --> b M' N
+  | red1r (b : op) C M M' N : 
+      C ||- M --> M' -> 
+      C ||- b N M --> b N M'
+where  "E '||-' t1 '-->' t2" := (red1 E t1 t2).
+
+
+Inductive conv (E : (evar_map * named_ctx * local_ctx)) (M : term) : term -> Prop :=
+  | conv_refl : conv E M M
+  | conv_trans1 P N : conv E M P -> red1 E P N -> conv E M N
+  | conv_trans1V P N : conv E M P -> red1 E N P -> conv E M N.
+
+Notation "E '||-' t '=?=' u" := (conv E t u) (at level 40). 
+
+
+Definition bhas_type (C : (evar_map * named_ctx * local_ctx)) (t1 t2 : term) :=
+  let: (E, N, L) := C in
+  match t1, t2 with
+  | Srt prop, Srt (kind _) => true
+  | Srt (kind i), Srt (kind j) => i <= j
+  | Bnd i, _ => if i < size L then t2 == (nth def_elem L i).2
+                else false
+  | Ref i, _ => if i \in map fst N then t2 == (get_def def_elem N i).2
+                else false
+  | _, _ => false
+  end.
+  
+
+
+(* TODO: missing acyclic test in evar_map *)
+Inductive has_type : (evar_map * named_ctx * local_ctx) -> term -> type -> Prop :=
+| TBase C t1 t2 : bhas_type C t1 t2 -> has_type C t1 t2
+(*| TAx1 E N L: 
+    (E, N, L) ||- Srt prop ~ Srt (kind 1)
+| TAx2 E N L i j:
+    i <= j -> 
+    (E, N, L) ||- Srt (kind i) ~ Srt (kind j)
+| TVar E N L i:
+    i < size L -> 
+    (E, N, L) ||- Bnd i ~ (nth def_elem L i).2
+| TConst E N L i:
+    i \in map fst N ->
+    (E, N, L) ||- Ref i ~ (get_def def_elem N i).2
+*)
+| TProd1 E N L T U s:
+    (E, N, L) ||- T ~ Srt s -> 
+    (E, N, (None, T) :: L) ||- U ~ Srt prop ->
+    (E, N, L) ||- Op Prod T U ~ Srt prop
+| TProd2 E N L T U i j k:
+    i <= k -> j <= k ->
+    (E, N, L) ||- T ~ Srt (kind i) -> 
+    (E, N, (None, T) :: L) ||- U ~ Srt (kind j) ->
+    (E, N, L) ||- Op Prod T U ~ Srt (kind k)
+| TLam E N L T t U s1 s2:
+    (E, N, L) ||- T ~ s1 -> 
+    (E, N, (None, T) :: L) ||- t ~ U ->
+    (E, N, L) ||- Op Prod T U ~ s2 ->
+    (E, N, L) ||- Op Abs T t ~ Op Prod T U
+| TApp C t u T U:
+    C ||- t ~ Op Prod U T ->
+    C ||- u ~ U ->
+    C ||- Op App t u ~ [db u]T 
+| TEvar E N L e d s T:
+    E.[e] = Some d ->
+    (E, N, L) ||-* s ~ d.(evar_ctx) ->
+    [n d.(evar_ctx) ::= s](d.(evar_concl)) = Some T ->
+    (E, N, L) ||- Evar e s ~ T
+| TConv E t T U : 
+    E ||- t ~ T ->
+    E ||- T =?= U ->
+    E ||- t ~ U
+with has_types : (evar_map * named_ctx * local_ctx) -> seq term -> named_ctx -> Prop :=  
+| CTId E : E ||-* [::] ~ [::]
+| CTAss E x t T T' s N :
+    E ||-* s ~ N ->
+    [n N ::= s]T = Some T' ->
+    E ||- t ~ T' ->
+    E ||-* (t :: s) ~ ((x, (None, T)) :: N)
+| CTDef E x t t' T T' s N :
+    E ||-* s ~ N ->
+    [n N ::= s]T = Some T' ->
+    E ||- t ~ T' ->
+    E ||- t =?= t' ->
+    E ||-* (t :: s) ~ ((x, (Some t', T)) :: N)
+where "E '||-' t '~' T" := (has_type E t T)
+and "E '||-*' s '~' N" := (has_types E s N).
+
+Definition wfE E := forall k v t, 
+  E.[k] = Some v -> 
+  (v.(evar_body) = None -> 
+   exists s, (E, v.(evar_ctx), [::]) ||- v.(evar_concl) ~ Srt s) /\ 
+  (v.(evar_body) = Some t -> 
+   (E, v.(evar_ctx), [::]) ||- t ~ v.(evar_concl)).
+
+Inductive wfN : evar_map -> named_ctx -> Prop :=
+| WFN0 E : wfN E [::]
+| WFNAss E (N : named_ctx) (x : ident) T s:
+    x \notin (map fst N) ->
+    (E, N, [::]) ||- T ~ Srt s ->
+    wfN E ((x, (None, T)) :: N)
+| WFNDef E (N : named_ctx) (x : ident) t T:
+    x \notin (map fst N) ->
+    (E, N, [::]) ||- t ~ T ->
+    wfN E ((x, (Some t, T)) :: N).
+
+Inductive wfL : (evar_map * named_ctx) -> local_ctx -> Prop :=
+| WFL0 E N : wfL (E, N) [::] 
+| WFLAss E N L T s: 
+    (E, N, L) ||- T ~ Srt s ->  
+    wfL (E, N) ((None, T) :: L)
+| WFLDef E N L t T: 
+    (E, N, L) ||- t ~ T ->  
+    wfL (E, N) ((Some t, T) :: L).
+
+Definition WF E N L := wfE E /\ wfN E N /\ wfL (E, N) L.
+
+Lemma get_def_weak d N i i' e : i != i' -> 
+  get_def d N i = get_def d ((i', e) :: N) i.
+Proof. by move=>H; rewrite {2}/get_def /= (negbTE H). Qed.
+Arguments get_def_weak [_ _ _] i' e _.
+
+Lemma weakeningN E N L t T i V : 
+  i \notin (map fst N) ->
+  (E, N, L) ||- t ~ T ->
+  (E, (i, V) :: N, L) ||- t ~ T.
+Proof.
+  move=>Hi H.
+  induction H. ; subst; try by constructor.
+  - rewrite (get_def_weak i V). apply TConst.
+  - case Hi0: (i0 \in (map fst N)).
+    rewrite /get_def.
+    
+  elim: t=>[s| n l | o t | | ] H.
+  - inversion H; subst; try by constructor.
+    apply (TConv H0 H1).
+Lemma wfL_ref E N L i t T: 
+  WF E N L -> (i, (Some t, T)) \in N -> 
+  (E, N, L) ||- t ~ T.
+Proof.
+  elim: N=>[//| [j [ot' T']] N' IH].
+  move=>H1 H2. move: H2 H1.
+  rewrite inE.
+  case/orP.
+  - move/eqP. case=><- <- <-.
+    move=>[WFE [WFN WFL]].
+    inversion WFN; subst.
+  move=>H1 H2.
+Theorem progress E t u T : 
+  E ||- t ~ T -> 
+  E ||- t --> u ->
+  E ||- u ~ T.
+Proof.
+elim; (try by (intros;
+              match goal with
+                  x : _ ||- _ --> _ |- _ => inversion x
+              end)); move: E=>_.
+- move=>E N L i.
+  move=>H1 H2 H3.
+  inversion H3; subst.
+  rewrite H8.
+  rewrite H8 in H2.
+  rewrite /= in H2 *.
+  inversion H2; subst.
