theories/ordtype.v
@@ -1,10 +1,54 @@
+(* Authors: Beta Ziliani and Cyril Cohen *)
 Require Import ssreflect ssrbool ssrnat eqtype ssrfun seq path fintype.
+
+(******************************************************************************)
+(* This files definies a totally ordered and decidable relations on a         *)
+(* type as canonical structure.  One need to import Order.Theory to get       *)
+(* the theory of such relations. The scope order_scope (%ord) contains        *)
+(* fancier notation for this kind of ordeeing.                                *)
+(*                                                                            *)
+(*           ordType == the type of ordered types                             *)
+(* OrdType ord_mixin == builds an ordtype from a mixing containing a proof of *)
+(*                             irreflexivity, transitivity and totality       *)
+(*                                                                            *)
+(* We provide a canonical structure of ordType for natural numbers (nat)      *)
+(* for finType and for pairs of ordType by lexicographic orderering.          *)
+(*                                                                            *)
+(* leP ltP ltgtP are the three main lemmas for case analysis, note that       *)
+(* they are doing a bit more than the one for natural numbers.                *)
+(*                                                                            *)
+(* We also provide specialized version of some theorems from path.v.          *)
+(*                                                                            *)
+(* There are three distinct uses of the symbols <, <=, > and >=:              *)
+(*    0-ary, unary (prefix) and binary (infix).                               *)
+(* 0. <%ord, <=%ord, >%ord, >=%ird stand respectively for lt, le, gt and ge.  *)
+(* 1. (< x),  (<= x), (> x),  (>= x) stand respectively for                   *)
+(*    (gt x), (ge x), (lt x), (le x).                                         *)
+(*    So (< x) is a predicate characterizing elements smaller than x.         *)
+(* 2. (x < y), (x <= y), ... mean what they are expected to.                  *)
+(*  These convention are compatible with haskell's,                           *)
+(*   where ((< y) x) = (x < y) = ((<) x y),                                   *)
+(*   except that we write <%R instead of (<).                                 *)
+(******************************************************************************)
+
 Set Implicit Arguments.
 Unset Strict Implicit.
 Import Prenex Implicits.
 
-Module Ordered. 
+Delimit Scope order_scope with ord.
+Local Open Scope order_scope.
 
+Reserved Notation "<= y" (at level 35).
+Reserved Notation ">= y" (at level 35).
+Reserved Notation "< y" (at level 35).
+Reserved Notation "> y" (at level 35).
+Reserved Notation "<= y :> T" (at level 35, y at next level).
+Reserved Notation ">= y :> T" (at level 35, y at next level).
+Reserved Notation "< y :> T" (at level 35, y at next level).
+Reserved Notation "> y :> T" (at level 35, y at next level).
+
+Module Order. 
+Module T.
 Section RawMixin.
 
 Structure mixin_of (T : eqType) := 
@@ -15,8 +59,6 @@ Structure mixin_of (T : eqType) :=
 
 End RawMixin.
 
-(* the class takes a naked type T and returns all the *)
-(* relatex mixins; the inherited ones and the added ones *)
 Section ClassDef.
 
 Record class_of (T : Type) := Class {
@@ -32,9 +74,6 @@ Variables (T : Type) (cT : type).
 Definition class := let: Pack _ c _ as cT' := cT return class_of cT' in c.
 Definition clone c of phant_id class c := @Pack T c T.
 
-(* produce an ordered type out of the inherited mixins *)
-(* equalize m0 and m by means of a phantom; will be exploited *)
-(* further down in the definition of OrdType *)
 Definition pack b (m0 : mixin_of (EqType T b)) := 
   fun m & phant_id m0 m => Pack (@Class T b m) T.
 
@@ -45,66 +84,252 @@ End ClassDef.
 Module Exports.
 Coercion sort : type >-> Sortclass.
 Coercion eqType : type >-> Equality.type.
-Canonical Structure eqType.
-Notation ordType := Ordered.type.
+Canonical eqType.
+Notation ordType := type.
 Notation OrdMixin := Mixin.
 Notation OrdType T m := (@pack T _ m _ id).
-Definition ord T : rel (sort T) := (ordering (mixin (class T))).
 Notation "[ 'ordType' 'of' T 'for' cT ]" := (@clone T cT _ id)
   (at level 0, format "[ 'ordType' 'of' T 'for' cT ]") : form_scope.
 Notation "[ 'ordType' 'of' T ]" := (@clone T _ _ id)
   (at level 0, format "[ 'ordType' 'of' T ]") : form_scope.
 End Exports.
-End Ordered.
-Export Ordered.Exports.
+End T.
+Import T.Exports.
 
-Prenex Implicits ord.
+Module Def.
+Section Def.
+Variable (T : ordType).
 
-Section Lemmas.
+Definition lt : rel T := (T.ordering (T.mixin (T.class T))).
+Local Notation "x < y" := (lt x y) : order_scope.
+
+Definition le : rel T := fun x y => (x == y) || (x < y).
+Local Notation "x <= y" := (le x y) : order_scope.
+
+Definition ge : simpl_rel T := [rel x y | y <= x].
+Definition gt : simpl_rel T := [rel x y | y < x].
+Definition leif x y C : Prop := ((x <= y) * ((x == y) = C))%type.
+Definition min x y : T := if x <= y then x else y.
+Definition max x y : T := if y <= x then x else y.
+
+Definition le_of_leif x y C (le_xy : @leif x y C) := le_xy.1 : le x y.
+
+End Def.
+End Def.
+
+Import Def.
+Prenex Implicits lt le leif min max.
+Notation lt := Def.lt.
+Notation le := Def.le.
+Notation gt := Def.gt.
+Notation ge := Def.ge.
+Notation leif := Def.leif.
+Notation min := Def.min.
+Notation max := Def.max.
+
+Module Import Syntax.
+
+Notation "<%ord" := lt : order_scope.
+Notation ">%ord" := gt : order_scope.
+Notation "<=%ord" := le : order_scope.
+Notation ">=%ord" := ge : order_scope.
+Notation "<?=%ord" := leif : order_scope.
+
+Notation "< y" := (gt y) : order_scope.
+Notation "< y :> T" := (< (y : T)) : order_scope.
+Notation "> y" := (lt y) : order_scope.
+Notation "> y :> T" := (> (y : T)) : order_scope.
+
+Notation "<= y" := (ge y) : order_scope.
+Notation "<= y :> T" := (<= (y : T)) : order_scope.
+Notation ">= y"  := (le y) : order_scope.
+Notation ">= y :> T" := (>= (y : T)) : order_scope.
+
+Notation "x < y"  := (lt x y) : order_scope.
+Notation "x < y :> T" := ((x : T) < (y : T)) : order_scope.
+Notation "x > y"  := (y < x) (only parsing) : order_scope.
+Notation "x > y :> T" := ((x : T) > (y : T)) (only parsing) : order_scope.
+
+Notation "x <= y" := (le x y) : order_scope.
+Notation "x <= y :> T" := ((x : T) <= (y : T)) : order_scope.
+Notation "x >= y" := (y <= x) (only parsing) : order_scope.
+Notation "x >= y :> T" := ((x : T) >= (y : T)) (only parsing) : order_scope.
+
+Notation "x <= y <= z" := ((x <= y) && (y <= z)) : order_scope.
+Notation "x < y <= z" := ((x < y) && (y <= z)) : order_scope.
+Notation "x <= y < z" := ((x <= y) && (y < z)) : order_scope.
+Notation "x < y < z" := ((x < y) && (y < z)) : order_scope.
+
+Notation "x <= y ?= 'iff' C" := (leif x y C) : order_scope.
+Notation "x <= y ?= 'iff' C :> R" := ((x : R) <= (y : R) ?= iff C)
+  (only parsing) : order_scope.
+
+Coercion le_of_leif : leif >-> is_true.
+End Syntax.
+
+Module Theory.
+Section Theory.
+
 Variable T : ordType.
+Implicit Types x y z : T.
 
-Lemma irr : irreflexive (@ord T). 
+Lemma lt_irreflexive : irreflexive (@lt T). 
+Proof. by case: T => s [b [m]]. Qed.
+
+Lemma ltxx x : x < x = false. Proof. exact: lt_irreflexive. Qed.
+
+Lemma lt_trans : transitive (@lt T). 
 Proof. by case: T=>s [b [m]]. Qed.
 
-Lemma trans : transitive (@ord T). 
-Proof. by case: T=>s [b [m]]. Qed.
+Lemma lt_total x y : [|| x < y, x == y | y < x]. 
+Proof. by case: T x y => s [b [m]]. Qed. 
 
-Lemma total (x y : T) : [|| ord x y, x == y | ord y x]. 
-Proof. by case: T x y=>s [b [m]]. Qed. 
+Lemma lexx x : x <= x. Proof. by rewrite /le eqxx. Qed.
 
-Lemma nsym (x y : T) : ord x y -> ord y x -> False.
-Proof. by move=>E1 E2; move: (trans E1 E2); rewrite irr. Qed. 
-
-End Lemmas. 
-
-Section Totality.
-Variable K : ordType.  
- 
-CoInductive total_spec (x y : K) : bool -> bool -> bool -> Type :=
-| total_spec_lt of ord x y : total_spec x y true false false
-| total_spec_eq of x == y : total_spec x y false true false
-| total_spec_gt of ord y x : total_spec x y false false true.
-
-Lemma totalP x y : total_spec x y (ord x y) (x == y) (ord y x).
+Lemma le_trans : transitive (@le T).
 Proof.
-case H1: (x == y).
-- by rewrite (eqP H1) irr; apply: total_spec_eq.
-case H2: (ord x y); case H3: (ord y x). 
-- by case: (nsym H2 H3). 
-- by apply: total_spec_lt H2.
-- by apply: total_spec_gt H3.
-by move: (total x y); rewrite H1 H2 H3.
+rewrite /le => y x z /predU1P [-> //|xy] yz; apply/orP; right.
+by move: yz => /predU1P [<- //|/(lt_trans xy) ->].
 Qed.
-End Totality. 
+
+Lemma ltW x y : x < y -> x <= y.
+Proof. by rewrite /le => ->; rewrite orbT. Qed.
+
+Lemma lt_nsym (x y : T) : lt x y -> lt y x -> False.
+Proof. by move=> xy /(lt_trans xy); rewrite ltxx. Qed.
+
+Hint Resolve lexx ltxx ltW.
+
+Lemma le_eqVlt x y : (x <= y) = (x == y) || (x < y). Proof. done. Qed.
+
+Lemma lt_neqAle x y : (x < y) = (x != y) && (x <= y).
+Proof. by rewrite /le; case: (altP eqP) => // ->. Qed.
+
+Lemma gt_eqF x y : y < x -> x == y = false.
+Proof. by apply: contraTF => /eqP ->; rewrite ltxx. Qed.
+
+Lemma lt_eqF x y : x < y -> x == y = false.
+Proof. by move=> hyx; rewrite eq_sym gt_eqF. Qed.
+
+CoInductive le_xor_gt (x y : T) : bool -> bool -> Set :=
+  | LerNotGt of x <= y : le_xor_gt x y true false
+  | GtrNotLe of y < x  : le_xor_gt x y false true.
+
+CoInductive lt_xor_ge (x y : T) : bool -> bool -> Set :=
+  | LtrNotGe of x < y  : lt_xor_ge x y false true
+  | GerNotLt of y <= x : lt_xor_ge x y true false.
+
+CoInductive comparer x y :
+  bool -> bool -> bool -> bool -> bool -> bool -> Set :=
+  | ComparerEq of x = y : comparer x y
+    true true true true false false
+  | ComparerLt of x < y : comparer x y
+    false false true false true false
+  | ComparerGt of x > y : comparer x y
+    false false false true false true.
+
+Lemma ltgtP x y :
+  comparer x y (y == x) (x == y) (x <= y) (y <= x) (x < y) (x > y).
+Proof.
+rewrite /le [y == x]eq_sym.
+have := (altP (x =P y), boolP (lt x y), boolP (lt y x), lt_total x y).
+rewrite /le => [] [[[[->|neq_xy]]]]; first by rewrite ltxx; constructor.
+by move=> [xy [/lt_nsym|]|? []] //=; constructor.
+Qed.
+
+Lemma leP x y : le_xor_gt x y (x <= y) (y < x).
+Proof. by have [->|xy|xy] := ltgtP; constructor => //; rewrite ltW. Qed.
+
+Lemma ltP x y : lt_xor_ge x y (y <= x) (x < y).
+Proof. by have [->|xy|xy] := ltgtP; constructor => //; rewrite ltW. Qed.
+
+Lemma le_total : total (@le T).
+Proof. by move=> x y; have [] := ltgtP. Qed.
+
+Hint Resolve le_total.
+
+Lemma le_asym : antisymmetric (le : rel T).
+Proof. by move=> x y; case: ltgtP. Qed.
+
+Lemma eq_le x y : (x == y) = (x <= y <= x).
+Proof. by apply/eqP/idP=> [->|/le_asym]; rewrite ?lexx. Qed.
+
+Lemma le_lt_trans y x z : x <= y -> y < z -> x < z.
+Proof. by rewrite !le_eqVlt => /orP[/eqP -> //|/lt_trans]; apply. Qed.
+
+Lemma lt_le_trans y x z : x < y -> y <= z -> x < z.
+Proof. by rewrite !le_eqVlt => lxy /orP[/eqP <- //|/(lt_trans lxy)]. Qed.
+
+Lemma leifP x y C : reflect (x <= y ?= iff C) (if C then x == y else x < y).
+Proof.
+rewrite /leif le_eqVlt; apply: (iffP idP)=> [|[]].
+  by case: C => [/eqP->|lxy]; rewrite ?eqxx // lxy lt_eqF.
+by move=> /orP[/eqP->|lxy] <-; rewrite ?eqxx // lt_eqF.
+Qed.
+
+Lemma lt_asym x y : x < y < x = false.
+Proof. by apply/negP=> /andP [/lt_trans hyx /hyx]; rewrite ltxx. Qed.
+
+Lemma le_anti : antisymmetric (@le T).
+Proof. by move=> x y; rewrite -eq_le=> /eqP. Qed.
+
+Lemma lt_le_asym x y : x < y <= x = false.
+Proof. by rewrite lt_neqAle -andbA -eq_le eq_sym; case: (_ == _). Qed.
+
+Lemma le_lt_asym x y : x <= y < x = false.
+Proof. by rewrite andbC lt_le_asym. Qed.
+
+Definition lter_anti := (=^~ eq_le, lt_asym, lt_le_asym, le_lt_asym).
+
+Lemma lt_geF x y : x < y -> (y <= x = false).
+Proof.
+by move=> xy; apply: contraTF isT=> /(lt_le_trans xy); rewrite ltxx.
+Qed.
+
+Lemma le_gtF x y : x <= y -> (y < x = false).
+Proof. by apply: contraTF=> /lt_geF->. Qed.
+
+Definition lt_gtF x y hxy := le_gtF (@ltW x y hxy).
+
+Lemma lt_sorted_uniq_le (s : seq T) :
+   sorted lt s = uniq s && sorted le s.
+Proof.
+case: s => //= n s; elim: s n => //= m s IHs n.
+rewrite inE lt_neqAle negb_or IHs -!andbA.
+case sn: (n \in s); last do !bool_congr.
+rewrite andbF; apply/and5P=> [[ne_nm lenm _ _ le_ms]]; case/negP: ne_nm.
+by rewrite eq_le lenm; apply: (allP (order_path_min le_trans le_ms)).
+Qed.
+
+Lemma sort_le_sorted (s : seq T) : sorted le (sort le s).
+Proof. by rewrite sort_sorted. Qed.
+
+Lemma eq_sorted_lt (s1 s2 : seq T) :
+  sorted lt s1 -> sorted lt s2 -> s1 =i s2 -> s1 = s2.
+Proof. by apply: eq_sorted_irr => //; apply: lt_trans. Qed.
+
+Lemma eq_sorted_le (s1 s2 : seq T) :
+   sorted le s1 -> sorted le s2 -> perm_eq s1 s2 -> s1 = s2.
+Proof. by apply: eq_sorted; [apply: le_trans|apply: le_anti]. Qed.
+
+Lemma sort_lt_sorted (s : seq T) : sorted lt (sort le s) = uniq s.
+Proof. by rewrite lt_sorted_uniq_le sort_uniq sort_le_sorted andbT. Qed.
+
+Lemma sort_le_id (s : seq T) : sorted le s -> sort le s = s.
+Proof.
+by move=> ss; apply: eq_sorted_le; rewrite ?sort_le_sorted // perm_sort.
+Qed.
+
+End Theory. 
 
 Section NatOrd.
-Lemma irr_ltn_nat : irreflexive ltn. Proof. by move=>x; rewrite /= ltnn. Qed.
-Lemma trans_ltn_nat : transitive ltn. Proof. by apply: ltn_trans. Qed.
-Lemma total_ltn_nat : forall x y, [|| x < y, x == y | y < x]. 
+Lemma irr_ltn_nat : irreflexive ltn. Proof. by move=> x; rewrite /= ltnn. Qed.
+Lemma trans_ltn_nat : transitive ltn. Proof. exact: ltn_trans. Qed.
+Lemma total_ltn_nat : forall x y, [|| x < y, x == y | y < x]%N. 
 Proof. by move=>*; case: ltngtP. Qed.
 
 Definition nat_ordMixin := OrdMixin irr_ltn_nat trans_ltn_nat total_ltn_nat.
-Canonical Structure nat_ordType := OrdType nat nat_ordMixin.
+Canonical nat_ordType := OrdType nat nat_ordMixin.
 End NatOrd.
 
 Section ProdOrd.
@@ -112,31 +337,26 @@ Variables K T : ordType.
 
 (* lexicographic ordering *)
 Definition lex : rel (K * T) := 
-  fun x y => if x.1 == y.1 then ord x.2 y.2 else ord x.1 y.1.
+  fun x y => if x.1 == y.1 then lt x.2 y.2 else lt x.1 y.1.
 
 Lemma irr_lex : irreflexive lex.
-Proof. by move=>x; rewrite /lex eq_refl irr. Qed.
+Proof. by move=>x; rewrite /lex eq_refl ltxx. Qed.
 
 Lemma trans_lex : transitive lex.
 Proof.
-move=>[x1 x2][y1 y2][z1 z2]; rewrite /lex /=.
-case: ifP=>H1; first by rewrite (eqP H1); case: eqP=>// _; apply: trans.
-case: ifP=>H2; first by rewrite (eqP H2) in H1 *; rewrite H1.
-case: ifP=>H3; last by apply: trans. 
-by rewrite (eqP H3)=>R1; move/(nsym R1).
+move=> [y1 y2] [x1 x2] [z1 z2]; rewrite /lex /=.
+have [->|_] := altP eqP; first by case: eqP => // _; apply: lt_trans.
+by have [-> xz|_ xy /(lt_trans xy) xz] := altP eqP; rewrite lt_eqF.
 Qed.
 
-Lemma total_lex : forall x y, [|| lex x y, x == y | lex y x].
+Lemma total_lex x y : [|| lex x y, x == y | lex y x].
 Proof.
-move=>[x1 x2][y1 y2]; rewrite /lex /=.
-case: ifP=>H1.
-- rewrite (eqP H1) eq_refl -pair_eqE /= eq_refl /=; exact: total.
-rewrite (eq_sym y1) -pair_eqE /= H1 /=.
-by move: (total x1 y1); rewrite H1.
+move: x y => [x1 x2] [y1 y2]; rewrite /lex /= -pair_eqE /=.
+by have [] //= := ltgtP x1 y1; have [] := ltgtP.
 Qed.
 
 Definition prod_ordMixin := OrdMixin irr_lex trans_lex total_lex.
-Canonical Structure prod_ordType := Eval hnf in OrdType (K * T) prod_ordMixin.
+Canonical prod_ordType := Eval hnf in OrdType (K * T) prod_ordMixin.
 End ProdOrd.
 
 Section FinTypeOrd.
@@ -146,24 +366,31 @@ Definition ordf : rel T :=
   fun x y => index x (enum T) < index y (enum T). 
 
 Lemma irr_ordf : irreflexive ordf.
-Proof. by move=>x; rewrite /ordf ltnn. Qed.
+Proof. by move=> x; rewrite /ordf ltxx. Qed.
 
 Lemma trans_ordf : transitive ordf.
-Proof. by move=>x y z; rewrite /ordf; apply: ltn_trans. Qed.
+Proof. by move=> x y z; rewrite /ordf; apply: ltn_trans. Qed.
 
-Lemma total_ordf : forall x y, [|| ordf x y, x == y | ordf y x].
+Lemma total_ordf x y : [|| ordf x y, x == y | ordf y x].
 Proof.
-move=>x y; rewrite /ordf; case: ltngtP=>//= H; rewrite ?orbT ?orbF //.
-have [H1 H2]: x \in enum T /\ y \in enum T by rewrite !mem_enum.
-by rewrite -(nth_index x H1) -(nth_index x H2) H eq_refl.
+rewrite /ordf; have [] := ltgtP; rewrite (orbT,orbF) //= => eq_xy.
+have [xT yT]: x \in enum T /\ y \in enum T by rewrite !mem_enum.
+by rewrite -(nth_index x xT) -(nth_index x yT) eq_xy eq_refl.
 Qed.
 
 Definition fin_ordMixin := OrdMixin irr_ordf trans_ordf total_ordf.
 End FinTypeOrd.
 
-(* notation to let us write I_n instead of (ordinal_finType n) *)
 Notation "[ 'fin_ordMixin' 'of' T ]" :=
-  (fin_ordMixin _ : Ordered.mixin_of [eqType of T]) (at level 0).
+  (fin_ordMixin _ : T.mixin_of [eqType of T]) (at level 0).
 
 Definition ordinal_ordMixin n := [fin_ordMixin of 'I_n].
-Canonical Structure ordinal_ordType n := OrdType 'I_n (ordinal_ordMixin n).
+Canonical ordinal_ordType n := OrdType 'I_n (ordinal_ordMixin n).
+
+Hint Resolve lexx ltxx ltW lt_irreflexive.
+Hint Resolve le_total le_trans le_anti lt_trans.
+
+End Theory.
+End Order.
+
+Export Order.T.Exports Order.Syntax.
